Make sure F* X64 semantics havocs flags in if/while, just like Dafny X64 semantics

fstar/code/arch/x64/X64.Vale.Decls.fst
@@ -44,6 +44,7 @@ let va_ins_lemma c0 s0 = ()
 
 let eval_ocmp = Lemmas.eval_ocmp
 let valid_ocmp = Lemmas.valid_ocmp
+let havoc = S.havoc
 
 unfold let va_eval_ins = Lemmas.eval_ins
 
